fixing compilation issues

Dafny/multisegment.dfy
@@ -2,46 +2,57 @@ include "segment.dfy"
 include "utils.dfy"
 module Multisegment{
 
+    import opened Segment
+    import opened Utils
+
     type Multisegment = seq<Segment>
 
 
-    predicate IsLadder(m : Multisegment){
-        exists enumeration : multisegment :: 
-            multiset(enumeration) = multiset(m) &&
+    ghost predicate IsLadder(m : Multisegment){
+        exists enumeration : Multisegment :: 
+            multiset(enumeration) == multiset(m) &&
+            |enumeration| == |m| &&
             forall index: int ::
                 0 <= index < |m| - 1 ==>
                     Precedes(enumeration[index], enumeration[index + 1])
     }
 
 
-    function depth(i : int, m : Multisegment): int
+    ghost function depth(i : int, m : Multisegment): int
         requires 0 <= i < |m|
     {
-        max(set s: seq<int> | |s| > 0 && multiset(s) <= multiset(m) && IsLadder(m) && s[0] = m[i] :: |s|-1)
+        MaxOf({0} + (set j: int | 0 <= j < |m| &&
+            exists s: seq<Segment> :: |s| == j + 1 && 
+            multiset(s) <= multiset(m) && IsLadder(s) && s[0] == m[i]))
     }
 
 
-    function d(m : Multisegment): int
+    ghost function d(m : Multisegment): int
         requires |m| > 0
     {
-        max(set index: int | 0 <= index < |m| :: depth(index, m))
+        MaxOf({0} + (set index: int | 0 <= index < |m| :: depth(index, m)))
     }
 
 
-    function bucket(m : Multisegment, k : int): set<int>
-        requires 0 <= k <= d(m)
+    ghost function bucket(m : Multisegment, k : int): set<int>
+        requires |m| > 0 && 0 <= k <= d(m)
     {
         set index: int | 0 <= index < |m| && depth(index, m) == k
     }
 
-    function AdmissibleEnumeration(m : Multisegment, k : int): seq<int>
+
+    ghost predicate IsAdmissibleEnumeration(m : Multisegment, k : int, enumeration : seq<int>)
         requires |m| > 0 && 0 <= k <= d(m)
-        {
-            var enumeration : seq<int> :| 
-                    SeqToSet(enumeration) == bucket(m, k)
-                    && (forall index: int :: 0 <= index < |enumeration| - 1 ==> 
-                        Precedes(m[enumeration[index+1]], m[enumeration[index]]));
-            enumeration
-        }
+    {
+        SeqToSet(enumeration) == bucket(m, k)
+        && (forall index : int :: 0 <= index < |enumeration| - 1 ==>
+            0 <= enumeration[index] < |m| &&
+            0 <= enumeration[index+1] < |m| &&
+            Precedes(m[enumeration[index+1]], m[enumeration[index]]))
+    }
+
+    ghost function {:axiom} AdmissibleEnumeration(m : Multisegment, k : int): (enumeration : seq<int>)
+        requires |m| > 0 && 0 <= k <= d(m)
+        ensures IsAdmissibleEnumeration(m, k, enumeration)
 
 }
