Dafny/segment.dfy
@@ -5,14 +5,14 @@ module Segment{
 
 
     method ShiftLeft(s : Segment) returns (s2 : Segment) {
-        s2 := (s.0 - 1, s.1 - 1)
+        s2 := (s.0 - 1, s.1 - 1);
     }
 
 
     method TruncateLeft(s : Segment) returns (s2 : Segment) 
         requires s.0 < s.1
     {
-        s2 := (s.0 + 1, s.1)
+        s2 := (s.0 + 1, s.1);
     }
 
 
@@ -24,5 +24,6 @@ module Segment{
     predicate SegSubsetEq(s1 : Segment, s2 : Segment){
         s1.0 <= s2.0 && s2.1 <= s1.1
     }
+ 
  
 }
